implemented agg_cnt, proof of init_maggaux and start of result_maggaux

thys/MFODL_Monitor_Devel/Optimized_Agg.thy
@@ -1,7 +1,113 @@
 theory Optimized_Agg
   imports Monitor
 begin
+type_synonym 'a agg_map = "(event_data tuple, 'a) mapping"
 
+datatype aggaux = CntAux "int agg_map" | SumAux "event_data table" | MinAux "event_data table"
+                    | MaxAux "event_data table" | AvgAux "event_data table" | MedAux "event_data table"
 
+fun valid_maggaux :: "aggargs \<Rightarrow> aggaux \<Rightarrow> event_data table \<Rightarrow> bool" where
+  "valid_maggaux \<lparr>aggargs_cols = cols, aggargs_n = n, aggargs_g0 = g0, aggargs_y = y, aggargs_\<omega> = \<omega>, aggargs_b = b, aggargs_f = f\<rparr> aux data = 
+  (let aggtype = fst \<omega> in case aux of 
+      CntAux m \<Rightarrow>
+        (aggtype = Formula.Agg_Cnt) \<and> (data = {} \<longleftrightarrow> Mapping.keys m = {}) \<and>
+        (\<forall>k. k \<in> (drop b) ` data \<longleftrightarrow> k \<in> Mapping.keys m) \<and>
+        (\<forall>k. k \<in> Mapping.keys m \<longrightarrow> Mapping.lookup m k = 
+          (let group = Set.filter (\<lambda>x. drop b x = k) data;
+           M = (\<lambda>y. (y, ecard (Set.filter (\<lambda>x. meval_trm f x = y) group))) ` meval_trm f ` group
+          in Some (length (flatten_multiset M))))
+    | SumAux t \<Rightarrow> (aggtype = Formula.Agg_Sum) \<and> t = data
+    | MinAux t \<Rightarrow> (aggtype = Formula.Agg_Min) \<and> t = data
+    | MaxAux t \<Rightarrow> (aggtype = Formula.Agg_Max) \<and> t = data
+    | AvgAux t \<Rightarrow> (aggtype = Formula.Agg_Avg) \<and> t = data
+    | MedAux t \<Rightarrow> (aggtype = Formula.Agg_Med) \<and> t = data)"
+
+fun init_maggaux :: "aggargs \<Rightarrow> aggaux" where
+  "init_maggaux args =
+  (let aggtype = fst (aggargs_\<omega> args) in case aggtype of
+      Formula.Agg_Cnt \<Rightarrow> CntAux Mapping.empty
+    | Formula.Agg_Sum \<Rightarrow> SumAux {}
+    | Formula.Agg_Min \<Rightarrow> MinAux {}
+    | Formula.Agg_Max \<Rightarrow> MaxAux {}
+    | Formula.Agg_Avg \<Rightarrow> AvgAux {}
+    | Formula.Agg_Med \<Rightarrow> MedAux {})"
+
+fun insert_maggaux :: "aggargs \<Rightarrow> event_data table \<Rightarrow> aggaux \<Rightarrow> aggaux" where
+  "insert_maggaux  \<lparr>aggargs_cols = cols, aggargs_n = n, aggargs_g0 = g0, aggargs_y = y, aggargs_\<omega> = \<omega>, aggargs_b = b, aggargs_f = f\<rparr> data aux = (case aux of
+    CntAux m \<Rightarrow> CntAux (foldl (\<lambda> m t. (let group = drop b t in case (Mapping.lookup m group) of
+                                       Some i \<Rightarrow> Mapping.update group (i + 1) m
+                                       | None \<Rightarrow> Mapping.update group 1 m) ) m (csorted_list_of_set data))
+  | SumAux t \<Rightarrow> SumAux (t \<union> data)
+  | MinAux t \<Rightarrow> MinAux (t \<union> data)
+  | MaxAux t \<Rightarrow> MaxAux (t \<union> data)
+  | AvgAux t \<Rightarrow> AvgAux (t \<union> data)
+  | MedAux t \<Rightarrow> MedAux (t \<union> data))"
+
+fun delete_maggaux :: "aggargs \<Rightarrow> event_data table \<Rightarrow> aggaux \<Rightarrow> aggaux" where
+  "delete_maggaux  \<lparr>aggargs_cols = cols, aggargs_n = n, aggargs_g0 = g0, aggargs_y = y, aggargs_\<omega> = \<omega>, aggargs_b = b, aggargs_f = f\<rparr> data aux = (case aux of
+    CntAux m \<Rightarrow> CntAux (foldl (\<lambda> m t. (let group = drop b t in case (Mapping.lookup m group) of
+                                       Some i \<Rightarrow> (if i = 1 then Mapping.delete group m 
+                                                  else Mapping.update group (i - 1) m)
+                                       | None \<Rightarrow> m) ) m (csorted_list_of_set data))
+  | SumAux t \<Rightarrow> SumAux (t - data)
+  | MinAux t \<Rightarrow> MinAux (t - data)
+  | MaxAux t \<Rightarrow> MaxAux (t - data)
+  | AvgAux t \<Rightarrow> AvgAux (t - data)
+  | MedAux t \<Rightarrow> MedAux (t - data))"
+
+fun result_maggaux :: "aggargs \<Rightarrow> aggaux \<Rightarrow> event_data table" where
+  "result_maggaux \<lparr>aggargs_cols = cols, aggargs_n = n, aggargs_g0 = g0, aggargs_y = y, aggargs_\<omega> = \<omega>, aggargs_b = b, aggargs_f = f\<rparr> aux = (case aux of
+    CntAux m \<Rightarrow> (if g0 \<and> Mapping.keys m = {} then singleton_table n y (eval_agg_op \<omega> {})
+    else (\<lambda>k. let agg_val = (EInt (integer_of_int (Mapping.lookup_default 0 m k))) in
+            k[y:=Some agg_val]) ` Mapping.keys m)
+  | SumAux t \<Rightarrow> eval_aggargs \<lparr>aggargs_cols = cols, aggargs_n = n, aggargs_g0 = g0, aggargs_y = y, aggargs_\<omega> = \<omega>, aggargs_b = b, aggargs_f = f\<rparr> t
+  | MinAux t \<Rightarrow> eval_aggargs \<lparr>aggargs_cols = cols, aggargs_n = n, aggargs_g0 = g0, aggargs_y = y, aggargs_\<omega> = \<omega>, aggargs_b = b, aggargs_f = f\<rparr> t
+  | MaxAux t \<Rightarrow> eval_aggargs \<lparr>aggargs_cols = cols, aggargs_n = n, aggargs_g0 = g0, aggargs_y = y, aggargs_\<omega> = \<omega>, aggargs_b = b, aggargs_f = f\<rparr> t
+  | AvgAux t \<Rightarrow> eval_aggargs \<lparr>aggargs_cols = cols, aggargs_n = n, aggargs_g0 = g0, aggargs_y = y, aggargs_\<omega> = \<omega>, aggargs_b = b, aggargs_f = f\<rparr> t
+  | MedAux t \<Rightarrow> eval_aggargs \<lparr>aggargs_cols = cols, aggargs_n = n, aggargs_g0 = g0, aggargs_y = y, aggargs_\<omega> = \<omega>, aggargs_b = b, aggargs_f = f\<rparr> t)"
+
+lemma valid_init_maggaux_unfolded: "safe_aggargs \<lparr>aggargs_cols = cols, aggargs_n = n, aggargs_g0 = g0, aggargs_y = y, aggargs_\<omega> = \<omega>, aggargs_b = b, aggargs_f = f\<rparr> \<Longrightarrow> valid_maggaux \<lparr>aggargs_cols = cols, aggargs_n = n, aggargs_g0 = g0, aggargs_y = y, aggargs_\<omega> = \<omega>, aggargs_b = b, aggargs_f = f\<rparr> (init_maggaux \<lparr>aggargs_cols = cols, aggargs_n = n, aggargs_g0 = g0, aggargs_y = y, aggargs_\<omega> = \<omega>, aggargs_b = b, aggargs_f = f\<rparr>) {}"
+  apply(induction "fst \<omega>")
+  by (auto)
+
+lemma valid_init_maggaux: "safe_aggargs args \<Longrightarrow> valid_maggaux args (init_maggaux args) {}"
+  using valid_init_maggaux_unfolded by (cases args) fast
+
+lemma valid_result_maggaux_unfolded: "valid_maggaux \<lparr>aggargs_cols = cols, aggargs_n = n, aggargs_g0 = g0, aggargs_y = y, aggargs_\<omega> = \<omega>, aggargs_b = b, aggargs_f = f\<rparr> aux X
+                                  \<Longrightarrow> result_maggaux \<lparr>aggargs_cols = cols, aggargs_n = n, aggargs_g0 = g0, aggargs_y = y, aggargs_\<omega> = \<omega>, aggargs_b = b, aggargs_f = f\<rparr> aux
+                                    = eval_aggargs \<lparr>aggargs_cols = cols, aggargs_n = n, aggargs_g0 = g0, aggargs_y = y, aggargs_\<omega> = \<omega>, aggargs_b = b, aggargs_f = f\<rparr> X"
+proof(induction aux)
+  case(SumAux x)
+  then show ?case by auto
+next 
+  case(MinAux x)
+  then show ?case by auto
+next
+  case(MaxAux x)
+  then show ?case by auto
+next
+  case(AvgAux x)
+  then show ?case by auto
+next  
+  case(MedAux x)
+  then show ?case by auto
+next
+  case(CntAux x)
+  from this have valid_agg: "valid_maggaux \<lparr>aggargs_cols = cols, aggargs_n = n, aggargs_g0 = g0, aggargs_y = y, aggargs_\<omega> = \<omega>, aggargs_b = b, aggargs_f = f\<rparr> (CntAux x) X"  by auto
+  then show ?case
+  proof (cases "g0 \<and> X = {}")
+    case(True)
+    then have assm: "g0 \<and> X = {}" by auto
+    have result_singleton: "result_maggaux \<lparr>aggargs_cols = cols, aggargs_n = n, aggargs_g0 = g0, aggargs_y = y, aggargs_\<omega> = \<omega>, aggargs_b = b, aggargs_f = f\<rparr> (CntAux x) = singleton_table n y (eval_agg_op \<omega> {})" 
+      using assm valid_agg by auto
+    have eval_singleton: "eval_aggargs \<lparr>aggargs_cols = cols, aggargs_n = n, aggargs_g0 = g0, aggargs_y = y, aggargs_\<omega> = \<omega>, aggargs_b = b, aggargs_f = f\<rparr> X = singleton_table n y (eval_agg_op \<omega> {})"
+      using assm unfolding eval_aggargs_def eval_agg_def by auto
+    show ?thesis using result_singleton eval_singleton by auto
+    case(False)
+    then have assm: "\<not>(g0 \<and> X = {})" by auto
+    have eval_subs_result: "eval_aggargs args X \<subseteq> result_maggaux args (CntAux x)" 
+    proof - {
+      
+    }
 
 end
